\documentclass{article}
\usepackage{amsmath}
\begin{document}

\begin{enumerate}
\item 1F-1
    \begin{enumerate}
        \item 
        \begin{equation*}
            f'(x) = 4x^3+8x
         \end{equation*}

        \item 
        \begin{equation*}
        f'(x) = 200x(x^2 + 2)^{99}
        \end{equation*}
    \end{enumerate}    
\item 1F-2
    \begin{align*}
        f'(x) &= x^9(x^2+1)^{10} + 20x^{11}(x^2+1)^9 \\
        &= x^9(x^2+1)^9((x^2+1) + 20x^2) \\
        &= x^9(x^2+1)^9(21x^2+1) \\
    \end{align*}
\item 1F-3
    if n is constant:
    \begin{equation*}
        f' = \frac{1}{n} x ^ \frac{1-n}{n}
    \end{equation*}
\item 1F-4
    \begin{align*}
        y &= (1 - x^{\frac{1}{3}})^3
    \end{align*}
    \begin{align*}
        y' &= 3(1-x^{\frac{1}{3}})^2 \\
        &= 3(1-x^{\frac{1}{3}})^2 \\
        &= x^{-\frac{2}{3}}(1-x^{\frac{1}{3}})^2
    \end{align*}
\item 1F-6
    if f(x) is even, $f(x) = f(-x)$:
    \begin{align*}
        f'(x) = \lim_{\Delta x \to 0} \frac{f(x+\Delta x) - f(x)}{\Delta x}
    \end{align*}
    \begin{align*}
        f'(-x) &= \lim_{\Delta x \to 0} \frac{f(-x+\Delta x) - f(-x)}{\Delta x} \\
                &= \lim_{\Delta x \to 0} \frac{f(-x+\Delta x) - f(x)}{\Delta x} \\
                &= \lim_{\Delta x \to 0} \frac{f(-(x-\Delta x)) - f(x)}{\Delta x} \\
                &= \lim_{\Delta x \to 0} \frac{f(x-\Delta x) - f(x)}{\Delta x} \\
    \end{align*}
\item 1F-7
    \begin{enumerate}
        \item 
            \begin{align*}
                \frac{dD}{dx} &= [(x-a)^2+y0^2]^{-\frac{1}{2}}(x-a)
            \end{align*}
        \item 
        \begin{align*}
            \frac{dm}{dv} 
            &= -\frac{1}{2}(1-\frac{v^2}{c^2})^{-\frac{3}{2}}(-\frac{2}{c^2}v) \\
            &= \frac{m0}{c^2}(1-\frac{v^2}{c^2})^{-\frac{3}{2}}v \\
        \end{align*}    
        \item
            \begin{align*}
                \frac{dF}{dr} &= (mg(1+r^2)^{-\frac{3}{2}})' \\
                &= 3mg(1+r^2)^{-\frac{5}{2}}r
            \end{align*}
        \item
            \begin{align*}
                \frac{dQ}{dt} = a(1+bt^2)^{-3}[1-3bt^2(1+bt^2)^{-1}]
            \end{align*}    
    \end{enumerate}
\end{enumerate}
\end{document}