\documentclass{article}
\usepackage{amsmath}
\begin{document}

\begin{enumerate}
\item 1E-1
    \begin{enumerate}
        \item 
        \begin{equation*}
            f'(x) = 10x^9 + 15x^2 + 6x^2
         \end{equation*}

        \item 
        \begin{equation*}
        f'(x) = 0
        \end{equation*}

        \item 
        \begin{equation*}
        f'(x) = \frac{1}{2}
        \end{equation*}

        \item 
        \begin{align*}
        f(x) &= x^8 + x^6 + x^5 + x^3 \\
        f'(x) &= 8x^7 + 6x^4 + 5x^4 + 3x^2
        \end{align*}
    \end{enumerate}    
\item 1E-2
    \begin{enumerate}

    \item 
    \begin{equation*}
        f(x) = \frac{a}{2}x^2 + bx
    \end{equation*}

    \item 
    \begin{equation*}
        f(x) = \frac{1}{7}x^7 + \frac{5}{6}x^6 + x^4
    \end{equation*}

    \item 
    \begin{align*}
        f'(x) &= x^6 + 2x^3 + 1 \\
        f(x) &= \frac{1}{7}x^7 + \frac{1}{2}x^4 + x
    \end{align*}
    \end{enumerate}
\item 1E-3
    \begin{equation*}
        y' = 3x^2 + 2x - 1
    \end{equation*}
    $3x^2 + 2x - 1 = 0$ at $x = \frac{1}{3}$ or $x = -1$,
    so the point is $(\frac{1}{3}, \frac{49}{27})$ or $(-1, 3)$
\item 1E-4
    \begin{enumerate}
        \item f(x) continuous at x = 0, 
        \begin{equation*}
            f'(x) = 
            \begin{cases}
                2ax + b <= 0 \\
                25x^4 + 12x^3 + 14x + 8 > 0
            \end{cases}
        \end{equation*}
        left limt = right limt at x = 0 so that b = 8. a can be any value.
        \item 
        \begin{equation*}
            f'(a) = 4a+5 \\
        \end{equation*}
    \end{enumerate}
\item 1E-5
    \begin{enumerate}
        \item 
            \begin{equation*}
                f'(x) = \frac{1}{(1+x)^2} \\
            \end{equation*}
        \item 
            \begin{equation*}
                f'(x) = \frac{-x^2 - 2ax + 1}{(x^2+1)^2} \\
            \end{equation*}
        \item 
            \begin{equation*}
                f'(x) = \frac{-x^2 -4x - 1}{(x^2-1)^2} \\
            \end{equation*}
        \item 
            \begin{equation*}
                f'(x) = \frac{3x^5 - x^4}{x^2} \\
            \end{equation*}            
    \end{enumerate}
\end{enumerate}


\end{document}