\documentclass{article}
\usepackage{amsmath}
\begin{document}

\begin{enumerate}
\item 1G-1
    \begin{enumerate}
        \item 
        \begin{equation*}
            f''(x) = 6-x^{-\frac{3}{2}}
         \end{equation*}

        \item 
        \begin{equation*}
        f''(x) = -10(x+5)^{-3}
        \end{equation*}

        \item 
        \begin{equation*}
        f''(x) = -10(x+5)^{-3}
        \end{equation*}

        \item 
        \begin{equation*}
        f''(x) = 0
        \end{equation*}
    \end{enumerate}    
\item 1G-2
    if $f''' = 0$ then $f'' = a$ and $a$ is constant, $f' = ax+b$ b is constant too. After that $f = \frac{a}{2}x^2+bx+c$ here c also constant.
\end{enumerate}
\end{document}