\documentclass{article}
\usepackage{amsmath}
\begin{document}

\begin{enumerate}
\item 1D-1
    \begin{enumerate}
        \item function continuie at x = 0.
        \begin{align*}
            \lim_{x \to 0} \frac{4}{x-1} = -4
        \end{align*}
        \item function continuie at x = 2.
        \begin{align*}
            \lim_{x \to 2} \frac{4x}{x+1} = \frac{8}{3}
        \end{align*}
        \item function not continuie at x = 2. undefined. 
        \item function not continuie at x = 2. going to $-\infty$ 
        \item function not continuie at x = 2. going to $+\infty$
        \item  
        \begin{align*}
            \lim_{x \to +\infty} \frac{4x^2}{x-2} = +\infty
        \end{align*}
        \item 
        \begin{align*}
            \lim_{x \to +\infty} \frac{4x^2}{x-2} - 4x &= \lim_{x \to +\infty} \frac{4x^2 - 4x^2 + 8x}{x-2} \\
            &= \lim_{x \to +\infty} \frac{8}{1-\frac{2}{x}} \\
            &= 8
        \end{align*}
        \item 
        \begin{align*}
            \lim_{x \to +\infty} \frac{x^2+2x+3}{3x^2-2x+4} &= \lim_{x \to +\infty} \frac{(1+\frac{2}{x}+\frac{3}{x^2})}{3 - \frac{2}{x} + \frac{4}{x^2}} \\
            &= \frac{1}{3}
        \end{align*}
        \item 
        \begin{align*}
            \lim_{x \to 2} \frac{x-2}{x^2-4} &= \lim_{x \to 2} \frac{x-2}{(x-2)(x+2)} \\
            &= \lim_{x \to 2} \frac{1}{x+2} \\
            &= \frac{1}{4}
        \end{align*}
    \end{enumerate}
\item 1D-2
    \begin{enumerate}
        \item 
            $\lim_{x \to 0+} \sqrt{x} = 0$, $\lim_{x \to 0-} \sqrt{x}$ is undefined
    \end{enumerate}
\item 1D-3
    \begin{enumerate}
        \item infinite discontinuity at $x = -2$
        \item infinite discontinuity at $x = 0 + k\pi$
        \item infinite discontinuity at x =0
        \item removable discontinuity at x =0
        \item jump discontinuity at x = 0 
        \item removable discontinuity at x = 0
    \end{enumerate}
\item 1D-5
    \begin{enumerate}
        \item 
            if f(x) continuous then $\lim_{x \to 1} f(x) = f(1)$
            \begin{equation*}
                \lim_{x \to 1-} x^2 = 1
            \end{equation*}
            \begin{equation*}
                \lim_{x \to 1+} ax+b = a
            \end{equation*}
            \begin{align*}
                \lim_{x \to 1-} &= \lim_{x \to 1+} \\
                 1 &= a
            \end{align*}
            $f(1) = b$, $b = 1$ too. and
            $a = 1, b = 1$
        \item 
            \begin{align*} f'(x) =
                \begin{cases}
                    a, x >= 1 \\
                    2x, x<1.
                \end{cases} 
            \end{align*}
            if f'(x) continuous then $\lim_{x \to 1} f'(x) = f'(1)$
            \begin{equation*}
                \lim_{x \to 1-} 2x = 2
            \end{equation*}
            \begin{equation*}
                \lim_{x \to 1+} a = a
            \end{equation*}
            so a = 2, $f'(1) = \lim_{x \to 1} f'(1)$
    \end{enumerate}
\item 1D-6
    \begin{enumerate}
        \item $f(x)$ is continuous at $x = 0$
            \begin{align*}
                \lim_{x \to 0}f(x) = f(0) \\
                \lim_{x \to 0-}f(x) = \lim_{x \to 0+}f(x)
            \end{align*} 
            \begin{align*}
                b = 1
                a = 4
            \end{align*}
        \item $f(x)$ is continuous at $x = 1$
            \begin{align*}
                \lim_{x \to 1}f(x) = f(1) \\
                \lim_{x \to 1-}f(x) = \lim_{x \to 1+}f(x) \\
                f'(1) = C
            \end{align*} 
            \begin{align*}
                a + b &= 6 \\
                b &= 0 \\
                a &= 6 \\
            \end{align*}
    \end{enumerate}
\end{enumerate}
\end{document}